ott_coq/destination_calculus_proofs.v
@@ -87,7 +87,7 @@ Proof.
     intros b. simpl. apply CtxM.add_1. reflexivity.
 Qed.
 
-Lemma SubLemma : forall (G1 G2 : ctx) (x : tmv) (m : mode) (T1 T2 : type) (t : term) (v : val), (G1 ⨄ ᶜ{ᵛ x ː m ‗ T2} ᵗ⊢ t ː T1) -> (G2 ᵗ⊢ term_Val v ː T2) -> mode_IsValid m -> ctx_IsValid (G1 ⨄ (m ᶜ· G2)) -> ((G1 ⨄ (m ᶜ· G2)) ᵗ⊢ t ᵗ[ x ≔ v ] ː T1).
+Lemma SubLemma : forall (G1 G2 : ctx) (x : var) (m : mode) (T1 T2 : type) (t : term) (v : val), (G1 ⨄ ᶜ{ᵛ x ː m ‗ T2} ᵗ⊢ t ː T1) -> (G2 ᵗ⊢ term_Val v ː T2) -> mode_IsValid m -> ctx_IsValid (G1 ⨄ (m ᶜ· G2)) -> ((G1 ⨄ (m ᶜ· G2)) ᵗ⊢ t ᵗ[ x ≔ v ] ː T1).
 Proof. Admitted.
 
 Axiom ProofAbsurd : forall (P : Prop), (~P -> False) -> P.
@@ -100,7 +100,7 @@ Axiom not_implies : forall (P Q : Prop), (~(P -> Q)) -> (P /\ ~Q).
 (* Missing ctx_DestOnly G in hypotheses? *)
 Theorem TypeSafety : forall (G : ctx) (t : term) (T : type), (G ᵗ⊢ t ː T) -> (forall (d : hddyn), exists (v : val) (e : eff), (t ‿ d ⇓ v ⋄ e) /\ (G ᶜ⊢ v ⋄ e ː T)).
 Proof.
-    intros G t T TYt. destruct TYt as [G t T TYRt ValidG NoHoleG]. induction TYRt.
+    intros G t T TYt. destruct TYt as [G t T TYt ValidG NoHoleG]. induction TYt.
     - (* TyR_term_H *) admit.
     - (* TyR_term_D *) admit.
     - (* TyR_term_U *) admit.
@@ -124,22 +124,22 @@ Proof.
         destruct NoHoleSG1G2 as [NoHoleSG1 NoHoleG2].
         assert (ctx_NoHole G1) as NoHoleG1. exact (StimesBackpropagatesNoHole m G1 NoHoleSG1).
         (* Get induction hypothesis and introduce v1 ⋄ e1 for t *)
-        assert (forall (d : hddyn), exists (v : val) (e : eff), (t ‿ d ⇓ v ⋄ e /\ G1 ᶜ⊢ v ⋄ e ː T1)) as TSt. exact (IHTYRt1 ValidG1 NoHoleG1).
+        assert (forall (d : hddyn), exists (v : val) (e : eff), (t ‿ d ⇓ v ⋄ e /\ G1 ᶜ⊢ v ⋄ e ː T1)) as TSt. exact (IHTYt1 ValidG1 NoHoleG1).
         destruct (TSt (d.1)) as [v1 TSt'].
         destruct TSt' as [e1 TSt''].
         destruct TSt'' as [REDt TYcmd1].
         (* Get induction hypothesis and introduce v2 ⋄ e2 for u *)
-        assert (forall (d : hddyn), exists (v : val) (e : eff), u ‿ d ⇓ v ⋄ e /\ G2 ᶜ⊢ v ⋄ e ː T1 ⁔ m → T2) as TSu. exact (IHTYRt2 ValidG2 NoHoleG2).
+        assert (forall (d : hddyn), exists (v : val) (e : eff), u ‿ d ⇓ v ⋄ e /\ G2 ᶜ⊢ v ⋄ e ː T1 ⁔ m → T2) as TSu. exact (IHTYt2 ValidG2 NoHoleG2).
         destruct (TSu (d.2)) as [v2 TSu'].
         destruct TSu' as [e2 TSu''].
         destruct TSu'' as [REDu TYcmd2].
         destruct TYcmd1 as [Ge1 Gv1 v1 e1 T1 TYe1 TYv1 DestOnlyGe1v1].
         destruct TYe1 as [Ge1 e1 TYRe1 ValidGe1].
-        dependent destruction TYv1. rename G into Gv1, T into T1, TYRt into TYRv1, H into ValidGv1, H0 into NoHoleGv1.
+        dependent destruction TYv1. rename G into Gv1, T into T1, TYt into TYRv1, H into ValidGv1, H0 into NoHoleGv1.
         dependent destruction TYcmd2. rename G1 into Ge2, G2 into Gv2, v into v2, e into e2, TYe into TYe2, TYv into TYv2, H into DestOnlyGe2v2.
         destruct TYe2 as [Ge2 e2 TYRe2 ValidGe2].
-        dependent destruction TYv2. rename G into Gv2, TYRt into TYRv2, H into ValidGv2, H0 into NoHoleGv2.
-        clear IHTYRt1. clear IHTYRt2. clear TSt. clear TSu.
+        dependent destruction TYv2. rename G into Gv2, TYt into TYRv2, H into ValidGv2, H0 into NoHoleGv2.
+        clear IHTYt1. clear IHTYt2. clear TSt. clear TSu.
         (* Canonical form on u *)
         inversion TYRv2.
             (* Prove that u : T1 ⁔ m → T2 cannot be a hole because its context is DestOnly *)
@@ -154,7 +154,7 @@ Proof.
               (* Proof that singleton contexts with two different bndr are not equal *)
               destruct H1 as (h0 & m0 & T & n & H1). unfold ctx_from_list, fold_right, ctx_add, bndr_name in H1. simpl in H1. unfold CtxM.add in H1. simpl in H1. congruence.
             (* Case where u is indeed a lambda value *)
-            * rename G into Gv2d, t0 into tb, T0 into T1d, m0 into md, T3 into T2d, TYRt into TYRtb, H2 into Validmd, H0 into Gv2dEqGv2, H into LamxtbEqv2, H1 into T1dEqT1, H3 into mdEqm, H4 into T2dEqT2.
+            * rename G into Gv2d, t0 into tb, T0 into T1d, m0 into md, T3 into T2d, TYt into TYtb, H2 into Validmd, H0 into Gv2dEqGv2, H into LamxtbEqv2, H1 into T1dEqT1, H3 into mdEqm, H4 into T2dEqT2.
               rewrite (eq_sym LamxtbEqv2) in TYRv2, REDu.
               clear mdEqm. clear Validmd. clear T1dEqT1. clear T2dEqT2. clear Gv2dEqGv2. clear md. clear Gv2d. clear T1d. clear T2d.  clear LamxtbEqv2. clear v2.
               assert (ctx_IsValid (m ᶜ· Gv1)) as ValidSGv1. exact (StimesPreservesValidity m Gv1 Validm ValidGv1).
@@ -173,7 +173,7 @@ Proof.
                 assert (ctx_IsValid ᶜ{ ᵛ x ː m ‗ T1}) as ValidXSing. unfold ctx_IsValid. intros n' b' MapsTo. unfold CtxM.MapsTo in MapsTo. simpl in MapsTo. unfold CtxM.Raw.PX.MapsTo in MapsTo. simpl in MapsTo. dependent destruction MapsTo. destruct H. simpl in H. simpl in H0. rewrite H0. simpl. exact Validm. inversion MapsTo.
                 assert (ctx_NoDest ᶜ{ ᵛ x ː m ‗ T1}) as NoDestXSing. unfold ctx_NoDest. intros n' b' MapsTo. unfold CtxM.MapsTo in MapsTo. simpl in MapsTo. unfold CtxM.Raw.PX.MapsTo in MapsTo. simpl in MapsTo. dependent destruction MapsTo. destruct H. simpl in H. simpl in H0. rewrite H0. unfold not. intros IsDest. dependent destruction IsDest. inversion MapsTo.
                 assert (ctx_NoHole ᶜ{ ᵛ x ː m ‗ T1}) as NoHoleXSing. unfold ctx_NoHole. intros n' b' MapsTo. unfold CtxM.MapsTo in MapsTo. simpl in MapsTo. unfold CtxM.Raw.PX.MapsTo in MapsTo. simpl in MapsTo. dependent destruction MapsTo. destruct H. simpl in H. simpl in H0. rewrite H0. unfold not. intros IsHole. dependent destruction IsHole. inversion MapsTo.
-              exact (SubLemma Gv2 Gv1 x m T2 T1 tb v1 (Ty_term_T (Gv2 ⨄ ᶜ{ ᵛ x ː m ‗ T1}) tb T2 TYRtb (UnionPreservesValidityDest Gv2 ᶜ{ ᵛ x ː m ‗ T1} ValidGv2 ValidXSing (InteractBackpropagatesDestOnly Ge2 Gv2 DestOnlyGe2v2) (NoDestXSing)) (UnionPreservesNoHole Gv2 (ᶜ{ ᵛ x ː m ‗ T1}) NoHoleGv2 NoHoleXSing)) (Ty_term_T Gv1 (term_Val v1) T1 TYRv1 ValidGv1 NoHoleGv1) Validm ValidGv2SGv1).
+              exact (SubLemma Gv2 Gv1 x m T2 T1 tb v1 (Ty_term_T (Gv2 ⨄ ᶜ{ ᵛ x ː m ‗ T1}) tb T2 TYtb (UnionPreservesValidityDest Gv2 ᶜ{ ᵛ x ː m ‗ T1} ValidGv2 ValidXSing (InteractBackpropagatesDestOnly Ge2 Gv2 DestOnlyGe2v2) (NoDestXSing)) (UnionPreservesNoHole Gv2 (ᶜ{ ᵛ x ː m ‗ T1}) NoHoleGv2 NoHoleXSing)) (Ty_term_T Gv1 (term_Val v1) T1 TYRv1 ValidGv1 NoHoleGv1) Validm ValidGv2SGv1).
 
               
               
